Weidenbach_Book/WB_List_More.thy
@@ -125,6 +125,15 @@ lemma Collect_minus_single_Collect: \<open>{x. P x} - {a} = {x . P x \<and> x \<
 lemma in_set_image_subsetD: \<open> f ` A \<subseteq> B \<Longrightarrow> x \<in> A \<Longrightarrow>f x \<in> B\<close>
   by blast
 
+lemma mset_tl:
+  \<open>mset (tl xs) = remove1_mset (hd xs) (mset xs)\<close>
+  by (cases xs) auto
+
+lemma hd_list_update_If:
+  \<open>outl' \<noteq> [] \<Longrightarrow> hd (outl'[i := w]) = (if i = 0 then w else hd outl')\<close>
+  by (cases outl') (auto split: nat.splits)
+
+
 text \<open>
   This lemma is not general enough to move to Isabelle, but might be interesting in other
   cases.\<close>
