Weidenbach_Book/WB_More_Refinement_List.thy
@@ -1,0 +1,92 @@
+theory WB_More_Refinement_List
+  imports Refine_Imperative_HOL.IICF Weidenbach_Book_Base.WB_List_More
+begin
+
+section \<open>More theorems about list\<close>
+
+text \<open>This should theorem and functions that defined in the Refinement Framework, but not in
+\<^theory>\<open>HOL.List\<close>. There might be moved somewhere eventually in the AFP or so.
+\<close>
+lemma swap_nth_irrelevant:
+  \<open>k \<noteq> i \<Longrightarrow> k \<noteq> j \<Longrightarrow> swap xs i j ! k = xs ! k\<close>
+  by (auto simp: swap_def)
+
+lemma swap_nth_relevant:
+  \<open>i < length xs \<Longrightarrow> j < length xs \<Longrightarrow> swap xs i j ! i = xs ! j\<close>
+  by (cases \<open>i = j\<close>) (auto simp: swap_def)
+
+lemma swap_nth_relevant2:
+  \<open>i < length xs \<Longrightarrow> j < length xs \<Longrightarrow> swap xs j i ! i = xs ! j\<close>
+  by (auto simp: swap_def)
+
+lemma swap_nth_if:
+  \<open>i < length xs \<Longrightarrow> j < length xs \<Longrightarrow> swap xs i j ! k =
+    (if k = i then xs ! j else if k = j then xs ! i else xs ! k)\<close>
+  by (auto simp: swap_def)
+
+lemma drop_swap_irrelevant:
+  \<open>k > i \<Longrightarrow> k > j \<Longrightarrow> drop k (swap outl' j i) = drop k outl'\<close>
+  by (subst list_eq_iff_nth_eq) auto
+
+lemma take_swap_relevant:
+  \<open>k > i \<Longrightarrow> k > j \<Longrightarrow>  take k (swap outl' j i) = swap (take k outl') i j\<close>
+  by (subst list_eq_iff_nth_eq) (auto simp: swap_def)
+
+lemma tl_swap_relevant:
+  \<open>i > 0 \<Longrightarrow> j > 0 \<Longrightarrow> tl (swap outl' j i) = swap (tl outl') (i - 1) (j - 1)\<close>
+  by (subst list_eq_iff_nth_eq)
+    (cases \<open>outl' = []\<close>; cases i; cases j; auto simp: swap_def tl_update_swap nth_tl)
+
+text \<open>TODO this should go to a different place from the previous lemmas, since it concerns
+\<^term>\<open>Misc.slice\<close>, which is not part of \<^theory>\<open>HOL.List\<close> but only part of the Refinement Framework.
+\<close>
+lemma slice_nth:
+  \<open>\<lbrakk>from \<le> length xs; i < to - from\<rbrakk> \<Longrightarrow> Misc.slice from to xs ! i = xs ! (from + i)\<close>
+  unfolding slice_def Misc.slice_def
+  apply (subst nth_take, assumption)
+  apply (subst nth_drop, assumption)
+  ..
+
+lemma slice_irrelevant[simp]:
+  \<open>i < from \<Longrightarrow> Misc.slice from to (xs[i := C]) = Misc.slice from to xs\<close>
+  \<open>i \<ge> to \<Longrightarrow> Misc.slice from to (xs[i := C]) = Misc.slice from to xs\<close>
+  \<open>i \<ge> to \<or> i < from \<Longrightarrow> Misc.slice from to (xs[i := C]) = Misc.slice from to xs\<close>
+  unfolding Misc.slice_def apply auto
+  by (metis drop_take take_update_cancel)+
+
+lemma slice_update_swap[simp]:
+  \<open>i < to \<Longrightarrow> i \<ge> from \<Longrightarrow> i < length xs \<Longrightarrow>
+     Misc.slice from to (xs[i := C]) = (Misc.slice from to xs)[(i - from) := C]\<close>
+  unfolding Misc.slice_def by (auto simp: drop_update_swap)
+
+lemma drop_slice[simp]:
+  \<open>drop n (Misc.slice from to xs) = Misc.slice (from + n) to xs\<close> for "from" n to xs
+    by (auto simp: Misc.slice_def drop_take ac_simps)
+
+lemma take_slice[simp]:
+  \<open>take n (Misc.slice from to xs) = Misc.slice from (min to (from + n)) xs\<close> for "from" n to xs
+  using antisym_conv by (fastforce simp: Misc.slice_def drop_take ac_simps min_def)
+
+lemma slice_append[simp]:
+  \<open>to \<le> length xs \<Longrightarrow> Misc.slice from to (xs @ ys) = Misc.slice from to xs\<close>
+  by (auto simp: Misc.slice_def)
+
+lemma slice_prepend[simp]:
+  \<open>from \<ge> length xs \<Longrightarrow>
+     Misc.slice from to (xs @ ys) = Misc.slice (from - length xs) (to - length xs) ys\<close>
+  by (auto simp: Misc.slice_def)
+
+lemma slice_len_min_If:
+  \<open>length (Misc.slice from to xs) =
+     (if from < length xs then min (length xs - from) (to - from) else 0)\<close>
+  unfolding min_def by (auto simp: Misc.slice_def)
+
+lemma slice_start0: \<open>Misc.slice 0 to xs = take to xs\<close>
+  unfolding Misc.slice_def
+  by auto
+
+lemma slice_end_length: \<open>n \<ge> length xs \<Longrightarrow> Misc.slice to n xs = drop to xs\<close>
+  unfolding Misc.slice_def
+  by auto
+
+end
